strengthened the spec of inner loop
outer loop has issues with definitional equality on types

examples/low-level/sieve.fst
@@ -54,42 +54,51 @@ type distinctRefsExists3
   (ra:ref a) (rb: ref b) (rc: ref c)  =
   (refExistsInMem ra m) /\ (refExistsInMem rb m) /\ (refExistsInMem rc m) /\ (ra=!=rb) /\ (rb=!=rc) /\ (ra=!=rc)
 
-type  innerLoopInv (n:nat) (lo: ref nat) (lov:nat) (li : ref nat) (res:ref ((k:nat{k<n}) -> Tot bool)) (m:smem) =
- distinctRefsExists3 m lo li res
+val markMultiplesUpto : n:nat -> lo:nat -> upto:nat{lo*(upto-1)<n}
+  ->((k:nat{k<n}) -> Tot bool) -> Tot ((k:nat{k<n}) -> Tot bool)
+let rec markMultiplesUpto n lo upto f =
+match upto with
+| 0 -> f
+| _ -> (mark n (markMultiplesUpto n lo (upto-1) f) ((upto-1)*lo))
+(* in below, markings are done in a reverse order as that of the while loop
+| _ -> markMultiplesUpto n lo (upto-1) (mark n f ((upto-1)*lo))*)
+
+type markedIffMultipleOrInit (n:nat) (lo:nat) (upto:nat{lo*(upto-1)<n})
+  (init:((k:nat{k<n}) -> Tot bool)) (new:((k:nat{k<n}) -> Tot bool)) =
+  (forall (k:nat{k < upto}). marked n new (lo*k))
+  /\ (forall (k:nat{k < n}). (marked n init k ==> marked n new k))
+  /\ (forall (k:nat{k < n}). (marked n new k ==> (marked n init k \/ divides lo k)))
+
+type  innerLoopInv (n:nat) (lo: ref nat) (lov:nat) (li : ref nat) (res:ref ((k:nat{k<n}) -> Tot bool))
+    (initres: ((k:nat{k<n}) -> Tot bool)) (m:smem) =
+ distinctRefsExists3 m lo res li
   /\ loopkupRef lo m = lov
-  /\ (((loopkupRef li m)-1)*(loopkupRef lo m) < n)
-  /\ (forall (k:nat).
-        (k < (loopkupRef li m)) ==> (marked n (loopkupRef res m) ((loopkupRef lo m)*k)))
+  /\ ((loopkupRef li m)-1)*lov < n
+  /\ markedIffMultipleOrInit n lov (loopkupRef li m) initres (loopkupRef res m)
+
+  (* this works, is totally precise, but is hard to use
+  /\ loopkupRef res m = markMultiplesUpto n lov (loopkupRef li m) initres*)
+
+        (*(k < (loopkupRef li m))
+            ==> (marked n (loopkupRef res m) ((loopkupRef lo m)*k)))*)
 
 type multiplesMarked2 (n:nat) (bitv : (k:nat{k<n}) -> Tot bool) (lo:nat) =
 (forall (k:nat). (k * lo < n)  ==> marked n bitv (lo*k))
 
+
+type markedIffDividesOrInit2 (n:nat) (lo:nat)
+  (init:((k:nat{k<n}) -> Tot bool)) (new:((k:nat{k<n}) -> Tot bool)) =
+  (forall (k:nat{k * lo < n}). marked n new (lo*k))
+  /\ (forall (k:nat{k < n}). (marked n init k ==> marked n new k))
+  /\ (forall (k:nat{k < n}). (marked n new k ==> (marked n init k \/ divides lo k)))
+
+
+ type markedIffDividesOrInit (n:nat) (lo:nat)
+   (init:((k:nat{k<n}) -> Tot bool)) (new:((k:nat{k<n}) -> Tot bool)) =
+    (forall (k:nat{k < n}). (marked n new k <==> (marked n init k \/ divides lo k)))
+
 type multiplesMarked (n:nat) (bitv : (k:nat{k<n}) -> Tot bool) (lo:nat) =
 (forall (m:nat{m<n}). (divides lo m) ==> marked n bitv m)
-
-val innerLoop : n:nat{n>1}
-  -> lo: ref nat
-  -> lov:nat
-  -> li : ref nat
-  -> res : ref ((k:nat{k<n}) -> Tot bool)
-  -> SST unit
-      (fun m -> distinctRefsExists3 m li lo res /\ loopkupRef li m = 0 /\ loopkupRef lo m = lov)
-      (fun m0 _ m1 -> distinctRefsExists3 m1 li lo res
-                      /\ loopkupRef lo m1 = lov
-                     /\ multiplesMarked n (loopkupRef res m1) (loopkupRef lo m1)
-      )
-let innerLoop n lo lov li res =
-  scopedWhile
-    (innerLoopInv n lo lov li res)
-    (innerGuardLC n lo li)
-    (fun u -> (memread li * memread lo < n))
-    (fun u ->
-      let liv = memread li in
-      let lov = memread lo in
-      let resv = memread res in
-      memwrite li (liv+1);
-      memwrite res (mark n resv (lov * liv)))
-
 
 val multiplesMarkedAsDivides :
   n:nat -> bitv:((k:nat{k<n}) -> Tot bool) -> lo:pos
@@ -97,6 +106,47 @@ val multiplesMarkedAsDivides :
     (requires (multiplesMarked2 n bitv lo))
     (ensures (multiplesMarked n bitv lo))
 let multiplesMarkedAsDivides n bitv lo = ()
+
+
+
+val multiplesMarkedAsDividesIff :
+  n:nat -> initv:((k:nat{k<n}) -> Tot bool) -> newv:((k:nat{k<n}) -> Tot bool) -> lo:pos
+  -> Lemma
+    (requires (markedIffDividesOrInit2 n lo initv newv))
+    (ensures (markedIffDividesOrInit n lo initv newv))
+let multiplesMarkedAsDividesIff n bitv newv lo = (multiplesMarkedAsDivides n newv lo)
+
+
+val innerLoop : n:nat{n>1}
+  -> lo: ref nat
+  -> lov:nat
+  -> li : ref nat
+  -> res : ref ((k:nat{k<n}) -> Tot bool)
+  -> initres : ((k:nat{k<n}) -> Tot bool)
+  -> SST unit
+      (requires (fun m ->
+        (*(refExistsInMem li m) /\ (refExistsInMem lo m) /\ (refExistsInMem res m) /\ (li=!=lo) /\ (lo=!=res) /\ (li=!=res)*)
+        distinctRefsExists3 m lo res li /\ loopkupRef li m = 0
+                    /\ loopkupRef lo m = lov /\ loopkupRef res m= initres))
+      (ensures (fun m0 _ m1 -> distinctRefsExists3 m1 lo res li
+                      /\ loopkupRef lo m1 = lov
+                     /\ markedIffDividesOrInit n (loopkupRef lo m1) initres (loopkupRef res m1)
+      ))
+
+let innerLoop n lo lov li res initres =
+  (scopedWhile
+    (innerLoopInv n lo lov li res initres)
+    (innerGuardLC n lo li)
+    (fun u -> (memread li * memread lo < n))
+    (fun u ->
+      let liv = memread li in
+      let lov = memread lo in
+      let resv = memread res in
+      memwrite li (liv+1);
+      memwrite res (mark n resv (lov * liv))));
+      (*the part below has no computaional content*)
+      let newv = memread res in
+      (multiplesMarkedAsDividesIff n initres newv lov)
 
 type distinctRefsExists2
   (#a:Type) (#b:Type) (m:smem)
@@ -112,34 +162,57 @@ type  outerLoopInv (n:nat) (lo: ref nat) (res:ref ((k:nat{k<n}) -> Tot bool)) (m
   /\ (((loopkupRef lo m) - 1) < n)
   /\ (1<(loopkupRef lo m))
   /\ (forall (k:nat).
-        (1<k /\ k < (loopkupRef lo m)) ==> multiplesMarked n (loopkupRef res m) k)
+        (1<k /\ k < (loopkupRef lo m)) ==> markedIffDividesOrInit n k (fun _ -> false) (loopkupRef res m))
 
-val outerLoop : n:nat{n>1}
-  -> lo: ref nat
-  -> res : ref ((k:nat{k<n}) -> Tot bool)
-  -> SST unit
-      (fun m -> distinctRefsExists2 m lo res /\ loopkupRef lo m =2)
-      (fun m0 _ m1 ->
-            distinctRefsExists2 m1 lo res
-           /\ (forall (k:nat).
-                (k < n ==> multiplesMarked n (loopkupRef res m1) k))
-      )
+val ex23 : #a:Type -> #b:Type  -> #c:Type -> m:smem
+  -> ra:ref a -> rb: ref b -> rc: ref c
+  -> Lemma
+        (requires (distinctRefsExists2 m ra rb /\ refExistsInMem rc m /\ (rc=!=ra) /\ (rc=!=rb)))
+        (ensures (distinctRefsExists3 m ra rb rc))
+let ex23 m ra rb rc = ()
 
-(*val factorialLoopBody :
+val ex23p : #a:Type -> #b:Type  -> #c:Type
+  -> ra:ref a -> rb: ref b -> rc: ref c
+  -> Lemma
+        (requires (True))
+        (ensures  ( forall m.
+                    ((distinctRefsExists2 (mtail m) ra rb /\ refExistsInMem rc m /\ (rc=!=ra) /\ (rc=!=rb)))
+                    ==> ((distinctRefsExists3 m ra rb rc))))
+let ex23p ra rb rc = ()
+
+#set-options "--initial_fuel 100 --max_fuel 10000 --initial_ifuel 100 --max_ifuel 10000"
+
+val factorialLoopBody :
   n:nat{n>1}
   -> lo:(ref nat)
   -> res : ref ((k:nat{k<n}) -> Tot bool)
   -> unit ->
-  whileBody (fun m -> b2t (refExistsInMem lo m)) (outerGuardLC n lo)
+  whileBody
+  (*SST unit*)
+    (fun m ->  distinctRefsExists2 m lo res)
+    (*(outerGuardLC n lo)*)
+    (fun  _ -> True)
+    (*(fun  _ _ _ -> True)*)
 
 let factorialLoopBody n lo res u =
-let li = salloc 0 in
-let resv = memread res in
-let lov = memread lo in
-innerLoop n lo lov li res;
-memwrite lo (lov+1)
+  (*pushStackFrame ();*)
+  let initres = memread res in
+  let lov = memread lo in
+  let li = salloc 0 in
+  let liv = memread li in
+  cut (liv==0);
+  cut (li=!=lo);
+  cut (li=!=res);
+  (ex23p lo res li);
+  (* innerLoop n lo lov li res initres*)
+  memwrite lo (lov+1)
+
+  (*popStackFrame ()*)
+
+
 
 effect SSTNull = SST unit (fun _ -> True) (fun _ _ _ -> True)
+
 
 val testSalloc1 : unit -> SST unit (fun _ -> True) (fun _ _ _ -> True)
 let testSalloc1 () =
@@ -158,8 +231,19 @@ let testSalloc2 xi =
 
 
 
+  val outerLoop : n:nat{n>1}
+    -> lo: ref nat
+    -> res : ref ((k:nat{k<n}) -> Tot bool)
+    -> SST unit
+        (fun m -> distinctRefsExists2 m lo res /\ loopkupRef lo m =2)
+        (fun m0 _ m1 ->
+              distinctRefsExists2 m1 lo res
+             /\ (forall (k:nat).
+                  (k < n ==> multiplesMarked n (loopkupRef res m1) k))
+        )
 
-let outerLoop n lo res =
+
+(*let outerLoop n lo res =
   scopedWhile
     (outerLoopInv n lo res)
     (outerGuardLC n lo)
@@ -168,6 +252,6 @@ let outerLoop n lo res =
       let li = salloc 0 in
       let resv = memread res in
       let lov = memread lo in
-      innerLoop n lo lov li res;
+      innerLoop n lo lov li res resv;
       memwrite lo (lov+1)
       )*)
